More baroque model

Flow.v
@@ -8,6 +8,17 @@ Local Open Scope string_scope.
 Local Open Scope Z_scope.
 Local Open Scope list_scope.
 
+Ltac HUNION :=
+  match goal with
+  | [ |- _ = hunion hempty _ ] =>
+      rewrite hunion_empty; HUNION
+  | [ |- _ = hunion _ hempty ] =>
+      rewrite hunion_comm; rewrite hunion_empty; HUNION
+  | _ => auto
+  end.
+
+Ltac heap := HUNION; HDISJ; auto.
+
 Module Flow3.
 
 Inductive flow : Type :=
@@ -18,14 +29,23 @@ Inductive flow : Type :=
 
 Infix ";;" := seq (at level 80, right associativity).
 
-Inductive satisfies : heap -> heap -> flow -> Prop :=
-  | sem_req: forall h3 p h1,
+Inductive result : Type :=
+| norm : Z -> result
+(* | eff : postcond -> flow *)
+.
+
+Inductive satisfies : bool -> heap -> bool -> heap -> result -> flow -> Prop :=
+  | sem_req: forall h3 p h1 r,
     (exists h2, h3 = hunion h1 h2 /\ hdisjoint h1 h2 /\ p h2) ->
-    satisfies h3 h1 (req p)
+    satisfies true h3 true h1 (norm r) (req p)
   | sem_ens: forall h1 h2 h3 q v,
     h3 = hunion h1 h2 -> hdisjoint h1 h2 ->
     q v h2 ->
-    satisfies h1 h3 (ens q)
+    satisfies true h1 true h3 (norm v) (ens q)
+  | sem_seq: forall f1 f2 r r1 h1 h2 h3 c,
+    satisfies true h1 true h2 r f1 ->
+    satisfies true h2 c h3 r1 f2 ->
+    satisfies true h1 c h3 r1 (f1;;f2)
 .
 
 (* forward rules. says how to produce a flow from a program *)
@@ -45,17 +65,20 @@ Definition terminated (c: com) : Prop :=  c = SKIP.
 Definition terminates (c1: com) (h1 h2: heap) : Prop :=
   exists c2, star red (c1, h1) (c2, h2) /\ terminated c2.
 
-Theorem soundness : forall f c1 h1 h2 h3,
-  satisfies h1 h3 f ->
-  forward c1 f ->
-  terminates c1 h1 h2 ->
+Theorem soundness : forall f e1 h1 h2 h3 c r,
+  satisfies true h1 c h3 r f ->
+  forward e1 f ->
+  terminates e1 h1 h2 ->
   h2 = h3.
 Proof.
-  intros f c1 h1 h2 h3 Hs.
+(* Abort. *)
+Proof.
+  intros f e1 h1 h2 h3 c r Hs.
   induction Hs; intros Hf Ht.
   - inv Hf.
   - { inv Hf.
-    - { inv Ht.
+    - {
+      inv Ht.
       admit.
     }
     (* - inv Ht. inv H0. inv H1. inv H2. inv H. inv H1. inv H0. rewrite hunion_comm. rewrite hunion_empty. auto. *)
@@ -65,5 +88,44 @@ Proof.
 Admitted.
 (* Qed. *)
 
+Example ex_spec_return_anything: exists x,
+  satisfies true hempty true hempty (norm x) (req emp).
+Proof.
+  exists 1.
+  constructor.
+  auto.
+  exists hempty.
+  repeat split; heap.
+Qed.
+
+Example ex_spec_ens_1:
+  satisfies true hempty true hempty (norm 1) (ens (fun r => (r = 1) //\\ emp)).
+Proof.
+  apply sem_ens with (h2 := hempty).
+  heap.
+  heap.
+  split.
+  auto. constructor.
+Qed.
+
+Example ex_spec_seq: forall x,
+  satisfies true (hupdate x 1 hempty) true (hupdate x 1 hempty) (norm 2)
+  (req (contains x 1);; ens (fun r => (r = 2) //\\ contains x 1)).
+Proof.
+  intros.
+  apply sem_seq with (h2 := hempty) (r := norm 3).
+  - constructor.
+  exists (hupdate x 1 hempty).
+  repeat split.
+  heap.
+  heap.
+  - apply sem_ens with (h2 := hupdate x 1 hempty).
+  heap.
+  heap.
+  split.
+  auto.
+  unfold contains.
+  reflexivity.
+Qed.
 
 End Flow3.
